general polishing of coq code; add also some structure for decomposition at the intermediate level

Intermediate/CS.v
@@ -6,6 +6,7 @@ Require Import CompCert.Smallstep.
 Require Import Common.Memory.
 Require Import Intermediate.Machine.
 Require Import Intermediate.GlobalEnv.
+Require Import Lib.Monads.
 
 Module CS.
   Import Intermediate.
@@ -14,76 +15,95 @@ Module CS.
 
   Definition state : Type := stack * Memory.t * Register.t * Pointer.t.
 
+  Definition initial_state
+             (G: global_env)
+             (mainC: Component.id) (mainP: Procedure.id)
+             (s: state) : Prop :=
+    let '(gps, mem, regs, pc) := s in
+    (* the global protected stack is empty *)
+    gps = [] /\
+    (* the program counter is pointing to the start of the main procedure *)
+    EntryPoint.get mainC mainP (genv_entrypoints G) = Some (Pointer.block pc) /\
+    Pointer.component pc = mainC /\
+    Pointer.offset pc = 0.
+
+  Definition final_state (G: global_env) (s: state) (r: int) : Prop :=
+    let '(gsp, mem, regs, pc) := s in
+    executing G pc IHalt.
+
   Inductive step (G : global_env) : state -> trace -> state -> Prop :=
   | Nop: forall gps mem regs pc,
-      executing G pc Nop ->
+      executing G pc INop ->
+      step G (gps, mem, regs, pc) E0 (gps, mem, regs, Pointer.inc pc)
+
+  | Label: forall gps mem regs pc l,
+      executing G pc (ILabel l) ->
       step G (gps, mem, regs, pc) E0 (gps, mem, regs, Pointer.inc pc)
 
   | Const: forall gps mem regs regs' pc r v,
-      executing G pc (Const v r) ->
+      executing G pc (IConst v r) ->
       Register.set r (imm_to_val v) regs = regs' ->
       step G (gps, mem, regs, pc) E0 (gps, mem, regs', Pointer.inc pc)
 
   | Mov: forall gps mem regs regs' pc r1 r2,
-      executing G pc (Mov r1 r2) ->
+      executing G pc (IMov r1 r2) ->
       Register.set r2 (Register.get r1 regs) regs = regs' ->
       step G (gps, mem, regs, pc) E0 (gps, mem, regs', Pointer.inc pc)
 
   | BinOp: forall gps mem regs regs' pc r1 r2 r3 op,
-      executing G pc (BinOp op r1 r2 r3) ->
+      executing G pc (IBinOp op r1 r2 r3) ->
       Register.set r3
                    (eval_binop op (Register.get r1 regs) (Register.get r2 regs))
                    regs = regs' ->
       step G (gps, mem, regs, pc) E0 (gps, mem, regs', Pointer.inc pc)
 
   | Load: forall gps mem regs regs' pc r1 r2 ptr v,
-      executing G pc (Load r1 r2) ->
+      executing G pc (ILoad r1 r2) ->
       Register.get r1 regs = Ptr ptr ->
       Memory.load mem ptr = Some v ->
       Register.set r2 v regs = regs' ->
       step G (gps, mem, regs, pc) E0 (gps, mem, regs', Pointer.inc pc)
 
   | Store: forall gps mem regs pc ptr r1 r2 mem',
-      executing G pc (Store r1 r2) ->
+      executing G pc (IStore r1 r2) ->
       Register.get r1 regs = Ptr ptr ->
       Pointer.component ptr = Pointer.component pc ->
       Memory.store mem ptr (Register.get r2 regs) = Some mem' ->
       step G (gps, mem, regs, pc) E0 (gps, mem', regs, Pointer.inc pc)
 
   | Jal: forall gps mem regs regs' pc pc' l,
-      executing G pc (Jal l) ->
+      executing G pc (IJal l) ->
       find_label_in_component G pc l = Some pc' ->
       Register.set R_RA (Ptr (Pointer.inc pc)) regs = regs' ->
       step G (gps, mem, regs, pc) E0 (gps, mem, regs', pc')
 
   | Jump: forall gps mem regs pc pc' r,
-      executing G pc (Jump r) ->
+      executing G pc (IJump r) ->
       Register.get r regs = Ptr pc' ->
       Pointer.component pc' = Pointer.component pc ->
       step G (gps, mem, regs, pc) E0 (gps, mem, regs, pc')
 
   | BnzNZ: forall gps mem regs pc pc' r l val,
-      executing G pc (Bnz r l) ->
+      executing G pc (IBnz r l) ->
       Register.get r regs = Int val ->
       val <> 0 ->
       find_label_in_procedure G pc l = Some pc' ->
       step G (gps, mem, regs, pc) E0 (gps, mem, regs, pc')
 
-  | BnzZ: forall gps mem regs pc pc' r l,
-      executing G pc (Bnz r l) ->
+  | BnzZ: forall gps mem regs pc r l,
+      executing G pc (IBnz r l) ->
       Register.get r regs = Int 0 ->
-      find_label_in_procedure G pc l = Some pc' ->
-      step G (gps, mem, regs, pc) E0 (gps, mem, regs, pc')
+      step G (gps, mem, regs, pc) E0 (gps, mem, regs, Pointer.inc pc)
 
   | Alloc: forall gps mem mem' regs regs' pc rsize rptr size ptr,
-      executing G pc (Alloc rptr rsize) ->
+      executing G pc (IAlloc rptr rsize) ->
       Register.get rsize regs = Int size ->
       Memory.alloc mem (Pointer.component pc) size = Some (mem', ptr) ->
       Register.set rptr (Ptr ptr) regs = regs' ->
       step G (gps, mem, regs, pc) E0 (gps, mem', regs', Pointer.inc pc)
 
   | Call: forall gps gps' mem regs pc b C' P rcomval,
-      executing G pc (Call C' P) ->
+      executing G pc (ICall C' P) ->
       Pointer.component pc <> C' ->
       imported_procedure (genv_interface G) (Pointer.component pc) C' P ->
       gps' = Pointer.inc pc :: gps ->
@@ -94,16 +114,163 @@ Module CS.
       step G (gps, mem, regs, pc) t (gps', mem, Register.invalidate regs, pc')
 
   | Return: forall gps gps' mem regs pc pc' rcomval,
-      executing G pc Return ->
+      executing G pc IReturn ->
       gps = pc' :: gps' ->
       Pointer.component pc <> Pointer.component pc' ->
       Register.get R_COM regs = Int rcomval ->
       let t := [ERet (Pointer.component pc) rcomval (Pointer.component pc')] in
       step G (gps, mem, regs, pc) t (gps', mem, Register.invalidate regs, pc').
 
-  Theorem determinism:
-    forall G s t s1 s2,
-      step G s t s1 -> step G s t s2 -> s1 = s2.
+  Section Semantics.
+    Variable p: program.
+    Variable mainC: Component.id.
+    Variable mainP: Procedure.id.
+
+    Definition sem :=
+      let G := init_env p in
+      @Semantics_gen state global_env step
+                     (initial_state G mainC mainP)
+                     (final_state G) G.
+  End Semantics.
+
+  Import MonadNotations.
+  Open Scope monad_scope.
+
+  Definition eval_step (G: global_env) (s: state) : option (trace * state) :=
+    let '(gps, mem, regs, pc) := s in
+    (* fetch the next instruction to execute *)
+    do C_procs <- NMap.find (Pointer.component pc) (genv_procedures G);
+    do P_code <- NMap.find (Pointer.block pc) C_procs;
+    do instr <- nth_error P_code (Pointer.offset pc);
+    (* decode and execute the instruction *)
+    match instr with
+    | ILabel l =>
+      ret (E0, (gps, mem, regs, Pointer.inc pc))
+    | INop =>
+      ret (E0, (gps, mem, regs, Pointer.inc pc))
+    | IConst v r =>
+      let regs' := Register.set r (imm_to_val v) regs in
+      ret (E0, (gps, mem, regs', Pointer.inc pc))
+    | IMov r1 r2 =>
+      let regs' := Register.set r2 (Register.get r1 regs) regs in
+      ret (E0, (gps, mem, regs', Pointer.inc pc))
+    | IBinOp op r1 r2 r3 =>
+      let regs' := Register.set
+                     r3 (eval_binop op (Register.get r1 regs) (Register.get r2 regs))
+                     regs in
+      ret (E0, (gps, mem, regs', Pointer.inc pc))
+    | ILoad r1 r2 =>
+      match Register.get r1 regs with
+      | Ptr ptr =>
+        do v <- Memory.load mem ptr;
+        let regs' := Register.set r2 v regs in
+        ret (E0, (gps, mem, regs', Pointer.inc pc))
+      | _ => None
+      end
+    | IStore r1 r2 =>
+      match Register.get r1 regs with
+      | Ptr ptr =>
+        if Pointer.component ptr =? Pointer.component pc then
+          do mem' <- Memory.store mem ptr (Register.get r2 regs);
+          ret (E0, (gps, mem', regs, Pointer.inc pc))
+        else
+          None
+      | _ => None
+      end
+    | IJal l =>
+      do pc' <- find_label_in_component G pc l;
+      let regs' :=  Register.set R_RA (Ptr (Pointer.inc pc)) regs in
+      ret (E0, (gps, mem, regs', Pointer.inc pc'))
+    | IJump r =>
+      match Register.get r regs with
+      | Ptr pc' =>
+        if Pointer.component pc' =? Pointer.component pc then
+          ret (E0, (gps, mem, regs, pc'))
+        else
+          None
+      | _ => None
+      end
+    | IBnz r l =>
+      match Register.get r regs with
+      | Int 0 =>
+        ret (E0, (gps, mem, regs, Pointer.inc pc))
+      | Int val =>
+        do pc' <- find_label_in_procedure G pc l;
+        ret (E0, (gps, mem, regs, pc'))
+      | _ => None
+      end
+    | IAlloc rptr rsize =>
+      match Register.get rsize regs with
+      | Int size =>
+        do (mem', ptr) <- Memory.alloc mem (Pointer.component pc) size;
+        let regs' := Register.set rptr (Ptr ptr) regs in 
+        ret (E0, (gps, mem', regs', Pointer.inc pc))
+      | _ => None
+      end
+    | ICall C' P =>
+      if negb (Pointer.component pc =? C') then
+        if imported_procedure_b (genv_interface G) (Pointer.component pc) C' P then
+          do b <- EntryPoint.get C' P (genv_entrypoints G);
+          match Register.get R_COM regs with
+          | Int rcomval =>
+            let pc' := (C', b, 0) in
+            let t := [ECall (Pointer.component pc) P rcomval C'] in
+            ret (t, (Pointer.inc pc :: gps, mem, Register.invalidate regs, pc'))
+          | _ => None
+          end
+        else
+          None
+      else
+        None
+    | IReturn =>
+      match gps with
+      | pc' :: gps' =>
+        if negb (Pointer.component pc =? Pointer.component pc') then
+          match Register.get R_COM regs with
+          | Int rcomval =>
+            let t := [ERet (Pointer.component pc) rcomval (Pointer.component pc')] in
+            ret (t, (gps', mem, Register.invalidate regs, pc'))
+          | _ => None
+          end
+        else
+          None
+      | _ => None
+      end
+    | IHalt => None
+    end.
+
+  Close Scope monad_scope.
+
+  Theorem eval_step_complete:
+    forall G st t st',
+      step G st t st' -> eval_step G st =  Some (t, st').
   Proof.
   Admitted.
+
+  Theorem eval_step_sound:
+    forall G st t st',
+      eval_step G st =  Some (t, st') -> step G st t st'.
+  Proof.
+  Admitted.
+
+  Theorem eval_step_correct:
+    forall G st t st',
+      eval_step G st =  Some (t, st') <-> step G st t st'.
+  Proof.
+    split.
+    apply eval_step_sound.
+    apply eval_step_complete.
+  Qed.
+
+  Theorem step_deterministic:
+    forall G st t st1 st2,
+      step G st t st1 -> step G st t st2 -> st1 = st2.
+  Proof.
+    intros G st t st1 st2 Hstep1 Hstep2.
+    apply eval_step_correct in Hstep1.
+    apply eval_step_correct in Hstep2.
+    rewrite Hstep1 in Hstep2.
+    inversion Hstep2.
+    reflexivity.
+  Qed.
 End CS.
