Intermediate/PS.v
@@ -1,8 +1,8 @@
 Require Import Common.Definitions.
 Require Import Common.Util.
+Require Import Common.Memory.
 Require Import CompCert.Events.
 Require Import CompCert.Smallstep.
-Require Import Common.Memory.
 Require Import Intermediate.Machine.
 Require Import Intermediate.GlobalEnv.
 Require Import Intermediate.CS.
@@ -19,9 +19,38 @@ Module PS.
   Definition program_state : Type := stack * Memory.t * Register.t * Pointer.t.
   Definition context_state : Type := stack * Memory.t * Component.id.
 
+  Inductive exec_state : Type := Normal | WentWrong | Halted.
+
   Inductive state : Type :=
   | PC : program_state -> state
-  | CC : context_state -> state.
+  | CC : context_state -> exec_state -> state.
+
+  Definition initial_state
+             (G: global_env)
+             (mainC: Component.id) (mainP: Procedure.id)
+             (s: state) : Prop :=
+    match s with
+    | PC (gps, mem, regs, pc) =>
+      (* the global protected stack is empty *)
+      gps = [] /\
+      (* the program counter is pointing to the start of the main procedure *)
+      EntryPoint.get mainC mainP (genv_entrypoints G) = Some (Pointer.block pc) /\
+      Pointer.component pc = mainC /\
+      Pointer.offset pc = 0
+    | CC (pgps, mem, C) execst =>
+      (* the global protected stack is empty *)
+      pgps = [] /\
+      (* the execution didn't go wrong *)
+      execst = Normal /\
+      (* the executing component is the main one *)
+      C = mainC
+    end.
+
+  Definition final_state (G: global_env) (s: state) (r: int) : Prop :=
+    match s with
+    | PC (gps, mem, regs, pc) => executing G pc IHalt
+    | CC (pgps, mem, C) execst => execst = Halted
+    end.
 
   Definition to_partial_frame pc frame : PartialPointer.t :=
     let '(C, b, o) := frame in
@@ -62,8 +91,8 @@ Module PS.
   Inductive step (G : global_env) : state -> trace -> state -> Prop :=
   | Program_Epsilon:
       forall gps pgps
-             (mem mem' wmem wmem' : Memory.t) cmem cmem'
-             (regs regs' : Register.t) (pc pc' : Pointer.t),
+        (mem mem' wmem wmem' : Memory.t) cmem cmem'
+        (regs regs' : Register.t) (pc pc' : Pointer.t),
         let C := Pointer.component pc in
         NMap.MapsTo C cmem wmem ->
         NMap.MapsTo C cmem' wmem' ->
@@ -74,7 +103,7 @@ Module PS.
 
   | Program_Internal_Call:
       forall pgps pgps' mem regs b o pc C' P val,
-        executing G pc (Call C' P) ->
+        executing G pc (ICall C' P) ->
         let C := Pointer.component pc in
         C' <> C ->
         imported_procedure (genv_interface G) C C' P ->
@@ -89,7 +118,7 @@ Module PS.
   | Program_Internal_Return:
       forall pgps pgps' mem regs pc pc' C' b o val,
         let C := Pointer.component pc in
-        executing G pc Return ->
+        executing G pc IReturn ->
         pgps = (C', Some (b,o)) :: pgps' ->
         C' <> C ->
         is_program_component G C' ->
@@ -100,29 +129,37 @@ Module PS.
   | Program_External_Call:
       forall pgps pgps' mem regs pc C' b o P val,
         let C := Pointer.component pc in
-        executing G pc (Call C' P) ->
+        executing G pc (ICall C' P) ->
         C' <> C ->
         imported_procedure (genv_interface G) C C' P ->
         is_context_component G C' ->
         pgps' = (C, Some (b,o)) :: pgps ->
         Register.get R_COM regs = Int val ->
         let t := [ECall C P val C'] in
-        step G (PC (pgps,mem,regs,pc)) t (CC (pgps',mem,C'))
+        step G (PC (pgps,mem,regs,pc)) t (CC (pgps',mem,C') Normal)
 
   | Program_External_Return:
       forall pgps pgps' mem regs pc C' val,
         let C := Pointer.component pc in
-        executing G pc Return ->
+        executing G pc IReturn ->
         C' <> C ->
         is_context_component G C' ->
         pgps = (C', None) :: pgps' ->
         Register.get R_COM regs = Int val ->
         let t := [ERet C val C'] in
-        step G (PC (pgps,mem,regs,pc)) t (CC (pgps',mem,C'))
+        step G (PC (pgps,mem,regs,pc)) t (CC (pgps',mem,C') Normal)
 
   | Context_Epsilon:
       forall pgps mem C,
-        step G (CC (pgps,mem,C)) E0 (CC (pgps,mem,C))
+        step G (CC (pgps,mem,C) Normal) E0 (CC (pgps,mem,C) Normal)
+
+  | Context_GoesWrong:
+      forall pgps mem C,
+        step G (CC (pgps,mem,C) Normal) E0 (CC (pgps,mem,C) WentWrong)
+
+  | Context_Halt:
+      forall pgps mem C,
+        step G (CC (pgps,mem,C) Normal) E0 (CC (pgps,mem,C) Halted)
 
   | Context_Internal_Call:
       forall pgps pgps' mem C C' P call_arg,
@@ -131,7 +168,7 @@ Module PS.
         is_context_component G C' ->
         pgps' = (C, None) :: pgps ->
         let t := [ECall C P call_arg C'] in
-        step G (CC (pgps,mem,C)) t (CC (pgps',mem,C'))
+        step G (CC (pgps,mem,C) Normal) t (CC (pgps',mem,C') Normal)
 
   | Context_Internal_Return:
       forall pgps pgps' mem C C' return_val,
@@ -139,7 +176,7 @@ Module PS.
         is_context_component G C' ->
         pgps = (C', None) :: pgps' ->
         let t := [ERet C return_val C'] in
-        step G (CC (pgps,mem,C)) t (CC (pgps',mem,C'))
+        step G (CC (pgps,mem,C) Normal) t (CC (pgps',mem,C') Normal)
 
   | Context_External_Call:
       forall pgps pgps' mem regs C C' P b val,
@@ -152,7 +189,7 @@ Module PS.
         Register.get R_COM regs = Int val ->
         let t := [ECall C P val C'] in
         let pc' := (C', b, 0) in
-        step G (CC (pgps,mem,C)) t (PC (pgps',mem,regs,pc'))
+        step G (CC (pgps,mem,C) Normal) t (PC (pgps',mem,regs,pc'))
 
   | Context_External_Return:
       forall pgps pgps' mem regs C C' b o val,
@@ -160,5 +197,28 @@ Module PS.
         is_program_component G C' ->
         Register.get R_COM regs = Int val ->
         let t := [ERet C val C'] in
-        step G (CC (pgps,mem,C)) t (PC (pgps',mem,regs, (C',b,o))).
+        step G (CC (pgps,mem,C) Normal) t (PC (pgps',mem,regs, (C',b,o))).
+
+  Definition partialize (p: program) (split: list Component.id) : program :=
+    {| prog_interface := prog_interface p;
+       prog_procedures :=
+         NMapExtra.filter
+           (fun C _ => negb (count_occ eq_nat_dec split C =? 0))
+           (prog_procedures p);
+       prog_buffers :=
+         NMapExtra.filter
+           (fun C _ => negb (count_occ eq_nat_dec split C =? 0))
+           (prog_buffers p) |}.
+
+  Section Semantics.
+    Variable p: program.
+    Variable mainC: Component.id.
+    Variable mainP: Procedure.id.
+
+    Definition sem :=
+      let G := init_env p in
+      @Semantics_gen state global_env step
+                     (initial_state G mainC mainP)
+                     (final_state G) G.
+  End Semantics.
 End PS.
