Intermediate/Decomposition.v
@@ -1,0 +1,54 @@
+Require Import Common.Definitions.
+Require Import Common.Util.
+Require Import Common.Memory.
+Require Import CompCert.Events.
+Require Import CompCert.Smallstep.
+Require Import Intermediate.Machine.
+Require Import Intermediate.GlobalEnv.
+Require Import Intermediate.CS.
+Require Import Intermediate.PS.
+
+Import Intermediate.
+
+Section Decomposition.
+  Variable p: program.
+  Variable mainC: Component.id.
+  Variable mainP: Procedure.id.
+  Variable split: list Component.id.
+
+  Let G := init_env p.
+  Let G' := init_env (PS.partialize p split).
+
+  Inductive related_states : CS.state -> PS.state -> Prop := .
+
+  Lemma initial_states_match:
+    forall s1,
+      CS.initial_state G mainC mainP s1 ->
+    exists s2,
+      PS.initial_state G' mainC mainP s2 /\ related_states s1 s2.
+  Proof.
+    intros s1 Hs1_init.
+    Admitted.
+
+  Lemma final_states_match:
+    forall s1 s2 r,
+      related_states s1 s2 ->
+      CS.final_state G s1 r -> PS.final_state G' s2 r.
+  Proof.
+  Admitted.
+
+  Lemma step_simulation:
+    forall s1 s2,
+      related_states s1 s2 ->
+    forall t s1',
+      CS.step G s1 t s1' ->
+    exists s2',
+      PS.step G' s2 t s2' /\ related_states s1' s2'.
+  Proof.
+  Admitted.
+
+  Theorem forward_sim:
+    forward_simulation (CS.sem p mainC mainP) (PS.sem (PS.partialize p split) mainC mainP).
+  Proof.
+  Admitted.
+End Decomposition.
