Source/Examples.v
@@ -3,10 +3,15 @@ Require Import Common.Values.
 Require Import Source.Language.
 Require Import Source.CS.
 Require Import Lib.Tactics.
+Require Import Lib.Monads.
 Require Import CompCert.Smallstep.
 Require Import CompCert.Events.
 
+Import MonadNotations.
+Open Scope monad_scope.
+
 Import Source.
+Import CS.
 
 (* naive factorial *)
 
@@ -18,7 +23,7 @@ Definition factorial : program := {|
                               Component.export := [1] |})];
   prog_buffers := NMapExtra.of_list [(1, 1); (2, 1)];
   prog_procedures := NMapExtra.of_list [
-    (1, NMapExtra.of_list [(0, E_call 2 0 (E_val (Int 3)))]);
+    (1, NMapExtra.of_list [(0, E_call 2 0 (E_val (Int 5)))]);
     (2, NMapExtra.of_list [(0,
       E_if (E_binop Leq (E_deref E_local) (E_val (Int 1)))
         (E_val (Int 1))
@@ -26,3 +31,32 @@ Definition factorial : program := {|
                  (E_deref E_local)
                  (E_call 2 0 (E_binop Minus (E_deref E_local) (E_val (Int 1))))))])]
 |}.
+
+(* this is super slow!!! it seems that maps are a problem *)
+(*
+Eval vm_compute in
+  do (G, st) <- init factorial 1 0;
+  match eval_kstep G st with
+  | None => None
+  | Some (_, (_, _, _, _, e)) => Some e
+  end.
+*)
+
+Definition example :=
+  (* warning (Int 1) is not considered at the moment *)
+  match run factorial (Int 1) 1000 with
+  | Some (_, _, _, _, E_val (Int n)) => Some n
+  | _ => None
+  end.
+
+(* Run with extraction to obtain a result *)
+(*
+let rec nat2int = function
+  | O -> 0
+  | S n -> 1 + nat2int n;;
+
+match example with
+| None -> print_string "error\n"
+| Some n -> print_int (nat2int n); print_newline ();;
+*)
+Extraction "/tmp/fact.ml" example.
