Source/PS.v
@@ -1,0 +1,13 @@
+Require Import Common.Definitions.
+Require Import Common.Util.
+Require Import Common.Values.
+Require Import Common.Memory.
+Require Import CompCert.Events.
+Require Import Source.Language.
+Require Import Source.GlobalEnv.
+
+Import Source.
+
+Module PS.
+
+End PS.
